# 10

The following procedure computes a mathematical function called Ackermann's function.
```
(define (A x y)
  (cond ((= y 0) 0)
	    ((= x 0) (* 2 y))
	    ((= y 1) 2)
	    (else (A (- x 1) (A x (- y 1))))))
```
What are the values of the following expressions?
```
(A 1 10)
(A 2 4)
(A 3 3)
```
Consider the following procedures, where `A` is the procedure defined above:
```
(define (f n) (A 0 n))
(define (g n) (A 1 n))
(define (h n) (A 2 n))
(define (k n) (* 5 n n))
```
Give concise mathematical definitions for the functions computed by the procedures `f`,`g`, and `h` for positive integer values of $n$. For example, `(k n)` computes $5n^2$.

## Solution

We evaluate the expression
```
1 ]=> (A 1 10)

(cond ((= 10 0) 0)
      ((= 1 0) (* 2 10))
      ((= 10 1) 2)
      (else (A (- 1 1) (A 1 (- 10 1)))))

(A (- 1 1) (A 1 (- 10 1)))

(A 0 (A 1 (- 10 1)))

(A 0 (A 1 9))

(A 0 (cond ((= 9 0) 0)
           ((= 1 0) (* 2 9))
           ((= 9 1) 2)
           (else (A (- 1 1) (A 1 (- 9 1))))))

(A 0 (A (- 1 1) (A 1 (- 9 1))))

(A 0 (A 0 (A 1 (- 9 1))))

(A 0 (A 0 (A 1 8)))
```
where we see the pattern, and the process expands as
```
(A 0 (A 0 (A 0 (A 1 7))))

(A 0 (A 0 (A 0 (A 0 (A 1 6)))))

(A 0 (A 0 (A 0 (A 0 (A 0 (A 1 5))))))

(A 0 (A 0 (A 0 (A 0 (A 0 (A 0 (A 1 4)))))))

(A 0 (A 0 (A 0 (A 0 (A 0 (A 0 (A 0 (A 1 3))))))))

(A 0 (A 0 (A 0 (A 0 (A 0 (A 0 (A 0 (A 0 (A 1 2)))))))))

(A 0 (A 0 (A 0 (A 0 (A 0 (A 0 (A 0 (A 0 (A 0 (A 1 1))))))))))

(A 0 (A 0 (A 0 (A 0 (A 0 (A 0 (A 0 (A 0 (A 0 (cond ((= 1 0) 0)
                                                   ((= 1 0) (* 2 1))
                                                   ((= 1 1) 2)
                                                   (else (A (- 1 1) (A 1 (- 1 1))))))))))))))

(A 0 (A 0 (A 0 (A 0 (A 0 (A 0 (A 0 (A 0 (A 0 2)))))))))

(A 0 (A 0 (A 0 (A 0 (A 0 (A 0 (A 0 (A 0 (cond ((= 2 0) 0)
                                              ((= 0 0) (* 2 2))
                                              ((= 2 1) 2)
                                              (else (A (- 0 1) (A 0 (- 2 1)))))))))))))

(A 0 (A 0 (A 0 (A 0 (A 0 (A 0 (A 0 (A 0 4))))))))
```
where we see the pattern, and the process contracts as
```
(A 0 (A 0 (A 0 (A 0 (A 0 (A 0 (A 0 8)))))))

(A 0 (A 0 (A 0 (A 0 (A 0 (A 0 16))))))

(A 0 (A 0 (A 0 (A 0 (A 0 32)))))

(A 0 (A 0 (A 0 (A 0 64))))

(A 0 (A 0 (A 0 128)))

(A 0 (A 0 256))

(A 0 512)

1 ]=> 1024
```

We evaluate the expression
```
1 ]=> (A 2 4)

(cond ((= 4 0) 0)
      ((= 2 0) (* 2 4))
      ((= 4 1) 2)
      (else (A (- 2 1) (A 2 (- 4 1)))))

(A (- 2 1) (A 2 (- 4 1)))

(A 1 (A 2 (- 4 1)))

(A 1 (A 2 3))

(A 1 (cond ((= 3 0) 0)
           ((= 2 0) (* 2 3))
           ((= 3 1) 2)
           (else (A (- 2 1) (A 2 (- 3 1))))

(A 1 (A (- 2 1) (A 2 (- 3 1))))

(A 1 (A 1 (A 2 (- 3 1))))

(A 1 (A 1 (A 2 2)))

(A 1 (A 1 (cond ((= 2 0) 0)
                ((= 2 0) (* 2 2))
                ((= 2 1) 2)
                (else (A (- 2 1) (A 2 (- 2 1)))))))

(A 1 (A 1 (A (- 2 1) (A 2 (- 2 1)))))

(A 1 (A 1 (A 1 (A 2 (- 2 1)))))

(A 1 (A 1 (A 1 (A 2 1))))

(A 1 (A 1 (A 1 (cond ((= 1 0) 0)
                     ((= 2 0) (* 2 1))
                     ((= 1 1) 2)
                     (else (A (- 2 1) (A 2 (- 1 1))))))))

(A 1 (A 1 (A 1 2)))

(A 1 (A 1 (cond ((= 2 0) 0)
                ((= 1 0) (* 2 2))
                ((= 2 1) 2)
                (else (A (- 1 1) (A 1 (- 2 1)))))))

(A 1 (A 1 (A (- 1 1) (A 1 (- 2 1)))))

(A 1 (A 1 (A 0 (A 1 (- 2 1)))))

(A 1 (A 1 (A 0 (A 1 1))))

(A 1 (A 1 (A 0 (cond ((= 1 0) 0)
                     ((= 1 0) (* 2 1))
                     ((= 1 1) 2)
                     (else (A (- 1 1) (A 1 (- 1 1))))))))

(A 1 (A 1 (A 0 2)))

(A 1 (A 1 (cond ((= 2 0) 0)
                ((= 0 0) (* 2 2))
                ((= 2 1) 2)
                (else (A (- 0 1) (A 0 (- 2 1)))))))

(A 1 (A 1 4))

(A 1 (cond ((= 4 0) 0)
           ((= 1 0) (* 2 4))
           ((= 4 1) 2)
           (else (A (- 1 1) (A 1 (- 4 1))))))

(A 1 (A (- 1 1) (A 1 (- 4 1))))

(A 1 (A 0 (A 1 (- 4 1))))

(A 1 (A 0 (A 1 3)))


```
